PSS: writing the final game transitions as x <-$- X\Y; ~ while (x \in Y) { x <-$- X; }
Adding some small examples to help in the development of the necessary functionalities.

examples/PSS.ec
@@ -800,7 +800,7 @@ section.
   by apply (G2_G3_abstract GAdv _); apply lossless_GAdv.
   qed.
 
-  (** TODO: Bound the probability of bad in G5 *)
+  (** TODO: Bound the probability of bad in G3 *)
 
   (** G4: compute z and u from the sampled values
         Note: z is uniform in "bitstrings of length k starting with a zero bit" (denoted '0 || 2^k-1'), and
@@ -867,7 +867,7 @@ section.
         by case (x{2} = x0); smt.
     by wp; skip; progress=> //; smt.
 
-    by if; [smt | | ]; wp; skip; progress=> //; smt.  
+    by if; [smt | | ]; wp; skip; progress=> //; smt.
   qed.
 
   local equiv G3_G4_abstract (Ga <: Gadv {H2,H3,G,Hmem}):
@@ -894,8 +894,44 @@ section.
   local equiv G3_G4: G3.main ~ G4.main: true ==> ={res}
   by apply (G3_G4_abstract GAdv).
 
-  (** G5: No longer using sk to simulate the oracles *)
+  (** G5: Sampling z in a (non-PTIME) loop *)
   local module H5: SplitOracle = {
+    fun init(ks:pkey * skey): unit = {
+      Hmap.init(ks);
+    }
+
+    fun o(c:bool,x:message * salt): htag = {
+      var b:bool;
+      var w:htag;
+      var st:gtag;
+      var z, u:signature;
+
+      b = true;
+      if (!in_dom x Hmap.m)
+      {
+        while (b)
+        {
+          z = $sample_plain Hmem.pk;
+          b = ((sub (to_bits z) 0 1) = ones 1);
+          w = HTag.from_bits (sub (to_bits z) 1 k1);
+          st = GTag.from_bits (sub (to_bits z) (k1 + 1) kg);
+          u = if c then ((inv Hmem.xstar Hmem.pk) * finv Hmem.sk  z) Hmem.pk else finv Hmem.sk z;
+          Hmap.m.[x] = (w,c,u);
+          G.m.[w] = st ^ (GTag.from_bits (to_bits (snd x) || zeros (kg - k0)));
+        }
+      }
+      else
+      {
+        if (!c /\ pi3_2 (proj Hmap.m.[x])) Hmap.m.[x] = (HTag.zeros,c,Signature.ones);
+      }
+      return pi3_1 (proj Hmap.m.[x]);
+    }
+  }.
+
+  local module G5 = Gen(GAdv,H5,G).
+
+  (** G6: upto "k2 executions of the loop didn't sample a bitstring starting with 0" *)
+  local module H6: SplitOracle = {
     var bad:bool
 
     fun init(ks:pkey * skey): unit = {
@@ -904,27 +940,29 @@ section.
     }
 
     fun o(c:bool,x:message * salt): htag = {
-      var b:bool = true;
-      var i:int = 0;
+      var b:bool;
       var w:htag;
       var st:gtag;
       var z, u:signature;
+      var i:int;
 
+      i = 0;
+      b = true;
       if (!in_dom x Hmap.m)
       {
-        while (i < kg2 && b)
+        while (b /\ i < kg2)
         {
-          u = $sample_plain Hmem.pk;
-          z = if c then (f Hmem.pk Hmem.xstar * f Hmem.pk u) Hmem.pk else f Hmem.pk u;
-          b = (sub (to_bits z) 0 1 = ones 1);
+          z = $sample_plain Hmem.pk;
+          b = ((sub (to_bits z) 0 1) = ones 1);
           w = HTag.from_bits (sub (to_bits z) 1 k1);
-          st = GTag.from_bits (sub (to_bits z) (k1 + 1) (kg));
-          i = i + 1;
+          st = GTag.from_bits (sub (to_bits z) (k1 + 1) kg);
+          u = if c then ((inv Hmem.xstar Hmem.pk) * finv Hmem.sk  z) Hmem.pk else finv Hmem.sk z;
           if (!b)
           {
             Hmap.m.[x] = (w,c,u);
             G.m.[w] = st ^ (GTag.from_bits (to_bits (snd x) || zeros (kg - k0)));
           }
+          i = i + 1;
         }
         bad = bad \/ b;
       }
@@ -936,7 +974,52 @@ section.
     }
   }.
 
-  local module G5 = Gen(GAdv,H5,G).
+  local module G6 = Gen(GAdv,H6,G).
+
+  (* G5_G6 will be a bit problematic because of the impossibility to synchronize the
+     loops unless an early exit is chosen *)
+
+  (** G7: No longer using sk to simulate the oracles *)
+  local module H7: SplitOracle = {
+    fun init(ks:pkey * skey): unit = {
+      Hmap.init(ks);
+    }
+
+    fun o(c:bool,x:message * salt): htag = {
+      var b:bool;
+      var w:htag;
+      var st:gtag;
+      var z, u:signature;
+      var i:int;
+
+      i = 0;
+      b = true;
+      if (!in_dom x Hmap.m)
+      {
+        while (b /\ i < kg2)
+        {
+          u = $sample_plain Hmem.pk;
+          z = if c then (f Hmem.pk Hmem.xstar * f Hmem.pk u) Hmem.pk else f Hmem.pk u;
+          b = (sub (to_bits z) 0 1 = ones 1);
+          w = HTag.from_bits (sub (to_bits z) 1 k1);
+          st = GTag.from_bits (sub (to_bits z) (k1 + 1) (kg));
+          if (!b)
+          {
+            Hmap.m.[x] = (w,c,u);
+            G.m.[w] = st ^ (GTag.from_bits (to_bits (snd x) || zeros (kg - k0)));
+          }
+          i = i + 1;
+        }
+      }
+      else
+      {
+        if (!c /\ pi3_2 (proj Hmap.m.[x])) Hmap.m.[x] = (HTag.zeros,c,Signature.ones);
+      }
+      return pi3_1 (proj Hmap.m.[x]);
+    }
+  }.
+
+  local module G7 = Gen(GAdv,H7,G).
 
   (** Reduction to OW: no longer using xstar to simulate the oracles *)
   local module I: Inverter = {
@@ -957,19 +1040,19 @@ section.
 
         if (!in_dom x m)
         {
-          while (i < kg2 && b)
+          while (b /\ i < kg2)
           {
             u = $sample_plain I.pk;
             z = if c then (ystar * f pk u) pk else f pk u;
             b = (sub (to_bits z) 0 1 = ones 1);
             w = HTag.from_bits (sub (to_bits z) 1 k1);
             st = GTag.from_bits (sub (to_bits z) (k1 + 1) (kg));
-            i = i + 1;
             if (!b)
             {
               m.[x] = (w,c,u);
               G.m.[w] = st ^ (GTag.from_bits (to_bits (snd x) || zeros (kg - k0)));
             }
+            i = i + 1;
           }
         }
         else
@@ -1029,7 +1112,7 @@ section.
             G.m.[w] = Some (sub ((f pk xstar) * (f pk u) [pk]) (k1 = 1) kg) ^ (r || zeros)
        There may also still be an upto bad step missing, that deals with the case where
        the adversary gets lucky and gets a valid signature out of fresh queries to H and G. *)
-  local equiv G5_OW_H: H5.o ~ I.H.o:
+  local equiv G7_OW_H: H7.o ~ I.H.o:
     ={glob G, x, c} /\
     Hmap.m{1} = I.H.m{2} /\
     Hmem.pk{1} = I.pk{2} /\
@@ -1039,19 +1122,13 @@ section.
     Hmem.pk{1} = I.pk{2} /\
     (f Hmem.pk Hmem.xstar){1} = I.ystar{2}.
   proof strict.
-  fun; inline H5.o I.H.o; wp; sp; if=> //.
+  fun; inline H7.o I.H.o; wp; sp; if=> //.
     wp; while (={glob G, i, b, c, x} /\
                Hmap.m{1} = I.H.m{2} /\
                Hmem.pk{1} = I.pk{2} /\
                (f Hmem.pk Hmem.xstar){1} = I.ystar{2})=> //.
-      seq 6 6: (={glob G, u, w, st, i, b, c, x} /\
-                Hmap.m{1} = I.H.m{2} /\
-                Hmem.pk{1} = I.pk{2} /\
-                (f Hmem.pk Hmem.xstar){1} = I.ystar{2} /\
-                i{1} <= kg2).
-        by wp; rnd; skip; smt.
-        by if; try wp.
-    by sp; if=> //; wp.
+          by wp; rnd; skip; smt.
+    by if=> //; wp.
   qed.
 end section.
 
